huge refactoring; attempt at an example program

theories/iris_examples.v
@@ -13,22 +13,40 @@ From iris.base_logic.lib Require Import gen_heap proph_map gen_inv_heap.
 From iris.program_logic Require Import weakestpre total_weakestpre.
 From iris.program_logic Require Export language lifting.
 
-Require Export common operations_iris datatypes_iris datatypes_properties_iris properties_iris.
-Require Import iris_locations iris.
+Require Import iris.
 
-Definition instance1 := 1.
-Definition instance2 := 2.
+Definition instance1 := 1%N.
+Definition instance2 := 2%N.
+Definition memory1 := 11%N.
+Definition byte1 := 21%N.
+Definition byte2 := 22%N.
 
 Definition store11 := list_byte_of_string "store11".
 Definition store42 := list_byte_of_string "store42".
 
 Notation "A ;;; B" := (HE_seq A B) (at level 2).
 Notation "A ::= B" := (HE_setglobal A B) (at level 5).
-(*
-Definition Program1 :=
-  10 ::= 
-  10 ::= (HE_new_rec [::(store11, )])
 
-Lemma example1:
-*)
-  
+Definition Program1 :=
+  (memory1 ::= (HE_wasm_memory_create 2 2 #00));;;
+  (byte1 ::= (HE_value (HV_byte #34)));;;
+  (byte2 ::= (HE_value (HV_byte #32)));;;
+  (HE_wasm_memory_set memory1 0%N byte1);;;
+  (HE_wasm_memory_set memory1 1%N byte2).
+
+Open Scope string_scope.
+Open Scope SEQ.
+
+Context `{!hsG Σ, !locG Σ, !wfuncG Σ, !wtabG Σ, !wmemG Σ, !wglobG Σ}.
+
+Lemma program1_spec s E:
+  ⊢
+  (WP Program1 @ s; E {{ v, (0%N ↦[wm][ 0%N ] #34) ∗ (0%N ↦[wm][ 1%N ] #32) }})%I.
+Proof.
+  repeat (iApply wp_seq; iSplitR).
+  iApply wp_setglobal_reduce; iSplitR.
+  iApply wp_mono; last by iApply wp_memory_create.
+  iIntros (v) "H".
+  destruct v => //; destruct w; try iAssumption; destruct m => //.
+  admit.
+Admitted.
