theories/stdpp_aux.v
@@ -1,0 +1,71 @@
+From mathcomp Require Import ssreflect ssrbool eqtype seq.
+
+Set Implicit Arguments.
+Unset Strict Implicit.
+Unset Printing Implicit Defensive.
+
+From stdpp Require Import gmap strings.
+Require Export common operations_iris datatypes_iris datatypes_properties_iris properties_iris.
+
+Lemma those_none: forall {T: Type} (l: list (option T)),
+  list_extra.those l = None <-> None ∈ l.
+Proof.
+  intros.
+  rewrite - list_extra.those_those0.
+  induction l => //=.
+  - split => //.
+    unfold elem_of.
+    move => HContra.
+    by inversion HContra.
+  - destruct a => //; rewrite elem_of_cons.
+    + unfold option_map.
+      destruct (those0 l) eqn:Hthose.
+      * split => //.
+        move => [H|H]; try by inversion H.
+        apply IHl in H.
+        by inversion H.
+      * split => //. intros _.
+        right. by apply IHl.
+    + split => //.
+      intros _. by left.
+Qed.
+
+Lemma those_length: forall {T: Type} (l: list (option T)) (le: list T),
+  list_extra.those l = Some le -> length l = length le.
+Proof.
+  move => T l le H.
+  rewrite - list_extra.those_those0 in H.
+  move: l le H.
+  induction l => //=.
+  - move => le H. simpl in H.
+    by inversion H.
+  - move => le H.
+    destruct a => //=.
+    unfold option_map in H.
+    destruct (those0 _) eqn:H2 => //=.
+    inversion H; subst; clear H.
+    simpl.
+    f_equal.
+    by apply IHl.
+Qed.
+
+Lemma those_lookup: forall {T: Type} (l: list (option T)) (le: list T) n,
+  list_extra.those l = Some le -> option_map (fun x => Some x) (le !! n) = l !! n.
+Proof.
+  move => T l le n Hthose.
+  rewrite - those_those0 in Hthose.
+  move : le n Hthose.
+  induction l => //=; move => le n Hthose.
+  - inversion Hthose; subst; clear Hthose.
+    unfold option_map.
+    by repeat rewrite list_lookup_empty.
+  - destruct a => //=.
+    unfold option_map in *.
+    destruct le => //=; first by destruct (those0 l).
+    destruct n => //=.
+    + destruct (those0 l) => //.
+      by inversion Hthose.
+    + destruct (those0 l) => //.
+      inversion Hthose; subst; clear Hthose.
+      by apply IHl. 
+Qed.
